Require constructor types to have the correct form

Defs.thy
@@ -41,6 +41,127 @@ proof goal_cases
 qed (auto simp: eqvt_def head_ctor_graph_aux_def)
 nominal_termination (eqvt) by lexicographic_order
 
+nominal_function ctor_data_app :: "\<tau> \<Rightarrow> (data_name * tyvar list) option" where
+  "ctor_data_app (TyVar _) = None"
+| "ctor_data_app (TyData T) = Some (T, [])"
+| "ctor_data_app TyArrow = None"
+| "ctor_data_app (TyApp \<tau>1 (TyVar a)) = (case ctor_data_app \<tau>1 of
+    Some (T, s) \<Rightarrow> Some (T, a#s)
+  | None \<Rightarrow> None)"
+| "ctor_data_app (TyApp _ (TyData _)) = None"
+| "ctor_data_app (TyApp _ TyArrow) = None"
+| "ctor_data_app (TyApp _ (TyApp _ _)) = None"
+| "ctor_data_app (TyApp _ (TyForall _ _ _)) = None"
+| "ctor_data_app (TyForall _ _ _) = None"
+proof goal_cases
+  case 1
+  then show ?case by (auto simp: eqvt_def ctor_data_app_graph_aux_def split!: option.splits)
+next
+  case (3 P x)
+  then show ?case
+  proof (cases x rule: \<tau>.exhaust)
+    case (TyApp \<tau>1 \<tau>2)
+    then show ?thesis using 3 by (cases \<tau>2 rule: \<tau>.exhaust) auto
+  qed (auto simp: 3)
+qed auto
+nominal_termination (eqvt) by lexicographic_order
+
+nominal_function ctor_type_app :: "\<tau> \<Rightarrow> (data_name * tyvar list) option" where
+  "ctor_type_app (TyVar _) = None"
+| "ctor_type_app (TyData T) = Some (T, [])"
+| "ctor_type_app TyArrow = None"
+| "ctor_type_app (TyApp (TyApp TyArrow \<tau>1) \<tau>2) = ctor_type_app \<tau>2"
+| "ctor_type_app (TyApp (TyApp (TyVar a) \<tau>1) \<tau>2) = ctor_data_app (TyApp (TyApp (TyVar a) \<tau>1) \<tau>2)"
+| "ctor_type_app (TyApp (TyApp (TyData T) \<tau>1) \<tau>2) = ctor_data_app (TyApp (TyApp (TyData T) \<tau>1) \<tau>2)"
+| "ctor_type_app (TyApp (TyApp (TyApp \<tau>1' \<tau>2') \<tau>1) \<tau>2) = ctor_data_app (TyApp (TyApp (TyApp \<tau>1' \<tau>2') \<tau>1) \<tau>2)"
+| "ctor_type_app (TyApp (TyApp (TyForall a k e) \<tau>1) \<tau>2) = ctor_data_app (TyApp (TyApp (TyForall a k e) \<tau>1) \<tau>2)"
+| "ctor_type_app (TyApp (TyVar a) \<tau>2) = ctor_data_app (TyApp (TyVar a) \<tau>2)"
+| "ctor_type_app (TyApp (TyData T) \<tau>2) = ctor_data_app (TyApp (TyData T) \<tau>2)"
+| "ctor_type_app (TyApp TyArrow \<tau>2) = ctor_data_app (TyApp TyArrow \<tau>2)"
+| "ctor_type_app (TyApp (TyForall a k e) \<tau>2) = ctor_data_app (TyApp (TyForall a k e) \<tau>2)"
+| "ctor_type_app (TyForall _ _ _) = None"
+proof goal_cases
+  case (3 P x)
+  show ?case using 3(1-3,13)
+  proof (cases x rule: \<tau>.exhaust)
+    case outer: (TyApp \<tau>1 \<tau>2)
+    then show ?thesis using 3(9-12)
+    proof (cases \<tau>1 rule: \<tau>.exhaust)
+      case inner: (TyApp \<tau>1' \<tau>2')
+      then show ?thesis using outer 3(4-8) by (cases \<tau>1' rule: \<tau>.exhaust) blast+
+    qed blast+
+  qed blast+
+next
+  case (74 a k e \<tau>1 \<tau>2 a k e \<tau>1 \<tau>2)
+  then show ?case by (simp add: 74)
+next
+  case (92 a k e \<tau>2 a k e \<tau>2)
+  then show ?case by (simp add: 92)
+qed (auto simp: eqvt_def ctor_type_app_graph_aux_def)
+nominal_termination (eqvt) by lexicographic_order
+
+nominal_function ctor_type_forall :: "\<tau> \<Rightarrow> (data_name * tyvar list) option" where
+  "ctor_type_forall (TyVar _) = None"
+| "ctor_type_forall (TyData T) = Some (T, [])"
+| "ctor_type_forall TyArrow = None"
+| "ctor_type_forall (TyApp \<tau>1 \<tau>2) = ctor_type_app (TyApp \<tau>1 \<tau>2)"
+| "ctor_type_forall (TyForall a _ e) = (case ctor_type_forall e of
+    Some (T, s) \<Rightarrow> (if a \<in> set s then Some (T, filter (\<lambda>x. x \<noteq> a) s) else None)
+  | None \<Rightarrow> None)"
+proof goal_cases
+  case 1
+  then show ?case by (auto simp: eqvt_def ctor_type_forall_graph_aux_def split!: option.splits list.splits)
+next
+  case (3 P x)
+  then show ?case by (cases x rule: \<tau>.exhaust)
+next
+  case (18 a k e a' k' e')
+  obtain c::tyvar where P: "atom c \<sharp> (a, e, a', e', ctor_type_forall_sumC e, ctor_type_forall_sumC e')" by (rule obtain_fresh)
+  then have c: "atom c \<sharp> a" "atom c \<sharp> e" "atom c \<sharp> a'" "atom c \<sharp> e'" "atom c \<sharp> ctor_type_forall_sumC e" "atom c \<sharp> ctor_type_forall_sumC e'" by auto
+  have 1: "(a \<leftrightarrow> c) \<bullet> e = (a' \<leftrightarrow> c) \<bullet> e'" using Abs_lst_rename_both c(1-4) 18(5) by auto
+  then have 2: "(a \<leftrightarrow> c) \<bullet> ctor_type_forall_sumC e = (a' \<leftrightarrow> c) \<bullet> ctor_type_forall_sumC e'" using 18(1,2) eqvt_at_def by metis
+  then have 3: "ctor_type_forall_sumC e = None \<longleftrightarrow> ctor_type_forall_sumC e' = None" using permute_eq_iff by fastforce
+  then show ?case
+  proof (cases "ctor_type_forall_sumC e")
+    case (Some t)
+    then obtain T s where P1: "t = (T, s)" by fastforce
+    from Some obtain T' s' where P2: "ctor_type_forall_sumC e' = Some (T', s')" using 3 by auto
+    have "T = T'" using "2" P1 P2 Some Some_eqvt option.inject perm_data_name_tyvar by auto
+    have same: "(a \<leftrightarrow> c) \<bullet> s = (a' \<leftrightarrow> c) \<bullet> s'" using "2" P1 P2 Some by auto
+    have x: "a \<in> set s \<longleftrightarrow> a' \<in> set s'" by (metis flip_at_simps(2) mem_permute_iff permute_flip_cancel same set_eqvt)
+    have 4: "atom c \<sharp> s" using c(5) Some P1 fresh_Some fresh_Pair by metis
+    have 5: "atom c \<sharp> s'" using c(6) Some P2 fresh_Some fresh_Pair by metis
+    have 6: "atom a \<sharp> filter (\<lambda>x. x \<noteq> a) s" "atom a' \<sharp> filter (\<lambda>x. x \<noteq> a') s'" "atom c \<sharp> filter (\<lambda>x. x \<noteq> a) s" "atom c \<sharp> filter (\<lambda>x. x \<noteq> a') s'" using 4 5 fresh_filter by auto
+    have 8: "filter (\<lambda>x. x \<noteq> a) s = (a \<leftrightarrow> c) \<bullet> filter (\<lambda>x. x \<noteq> a) s" using 6 flip_fresh_fresh by metis
+    also have "... = filter (\<lambda>x. x \<noteq> c) ((a \<leftrightarrow> c) \<bullet> s)" by auto
+    also have "... = filter (\<lambda>x. x \<noteq> c) ((a' \<leftrightarrow> c) \<bullet> s')" using same by argo
+    also have "... = (a' \<leftrightarrow> c) \<bullet> filter (\<lambda>x. x \<noteq> a') s'" by simp
+    also have "... = filter (\<lambda>x. x \<noteq> a') s'" using 6 flip_fresh_fresh by blast
+    finally have 9: "Some (T, filter (\<lambda>x. x \<noteq> a) s) = Some (T', filter (\<lambda>x. x \<noteq> a') s')" using \<open>T = T'\<close> by blast
+    then show ?thesis using Some P1 P2 x by simp
+  qed simp
+qed auto
+nominal_termination (eqvt) by lexicographic_order
+
+(* This function checks if a type has the form \<forall>[a:k]. [\<tau>] \<rightarrow> T [a] *)
+nominal_function ctor_type :: "\<tau> \<Rightarrow> data_name option" where
+  "ctor_type (TyVar a) = None"
+| "ctor_type (TyData T) = Some T"
+| "ctor_type TyArrow = None"
+| "ctor_type (TyApp \<tau>1 \<tau>2) = (case ctor_type_app (TyApp \<tau>1 \<tau>2) of Some (T, []) \<Rightarrow> Some T | _ \<Rightarrow> None)"
+| "ctor_type (TyForall a k e) = (case ctor_type_forall (TyForall a k e) of Some (T, []) \<Rightarrow> Some T | _ \<Rightarrow> None)"
+proof goal_cases
+  case 1
+  then show ?case by (auto simp: eqvt_def ctor_type_graph_aux_def split!: option.splits list.splits)
+next
+  case (3 P x)
+  then show ?case by (cases x rule: \<tau>.exhaust)
+next
+  case (18 a k e a' k' e')
+  then show ?case by (simp add: 18)
+qed auto
+nominal_termination (eqvt) by lexicographic_order
+
 nominal_function is_value :: "term => bool" where
   "is_value (Var x) = False"
 | "is_value (\<lambda> x : \<tau> . e) = True"
